# Q1

## a

$$
Im(z) = -2; 
$$

It's the vertical line where y = 2. 

## b

$$
|z-1+i|=3
$$

it's a circle with the radius 3 and center (1, -1)

# 2

If $Arg(z_1) = Arg(z_2)$, that means there are in the same direction, then length of the sum is the sum of the length, reverse is true. 

# 3

$$
e^{i\theta} = cos(\theta) + isin(\theta) \\
e^{-i\theta} = cos(-\theta) + isin(-\theta) = cos(\theta) - isin(\theta) \\
cos(\theta) = \frac{(e^{i\theta} + e^{-i\theta})}{2} \\
sin(\theta) = \frac{(e^{i\theta} - e^{-i\theta})}{2i} \\
tan(\theta) = \frac{sin(\theta)}{cos(\theta)} = \frac{e^{i\theta} - e^{-i\theta}}{i(e^{i\theta} + e^{-i\theta})}
$$

# 4

## a

$$
2z^2 + z+3=0
$$

$$
z = \frac{-1 \pm \sqrt{1 - 4 * 2 * 3}}{4} = -\frac{1}{4} \pm \frac{\sqrt{23}i}{4}
$$

## b

$$
z^2 - (3-2i)z+(1-3i) = 0
$$

$$
z = \frac{(3-2i) \pm \sqrt{(3-2i)^2 - 4(1-3i)}}{2} = \frac{(3-2i) \pm \frac{e^{1/2}}{\sqrt{17}} (1+4i) }{2}
$$

## c

$$
z^2 - 2z + i = 0
$$

$$
z = \frac{2 \pm \sqrt{4 - 4i}}{2} = 1 \pm \sqrt{1-i}
$$

# 5

$$
\frac{\part u}{\part x} = \frac{2x}{x^2 + y^2}
$$

$$
u = \frac{2(y^2 - x^2)}{(x^2 + y ^ 2)^2} + \phi(y) \\
\phi(y) = 0 \\
u = \frac{2(y^2 - x^2)}{(x^2 + y ^ 2)^2} + C
$$

# 6

## a

$$
\frac{a}{1-c} + i\frac{b}{1-c} = i \\
P = (0, 1, 0)
$$

## b

$$
\frac{a}{1-c} + i\frac{b}{1-c} = 6 - 8i \\
a^2 + b^2 + c^2 = 1
$$

## c

$$
\frac{a}{1-c} + i\frac{b}{1-c} = -\frac{3}{10} + \frac{2}{5}i \\
a^2 + b^2 + c^2 = 1
$$

# 7

## a

$$
\begin{align}
f(z) & = 3z^2 + 5z + i + 1 \\ 
& = 3(x^2 -y^2 + 2ixy) + 5(x+ iy) + i + 1 \\
& = (3x^2 - 3y^2 + 5x + 1) + i(6xy + 5y + 1)
\end{align}
$$

## b

$$
g(z) = 1/z = \frac{1}{x + iy} = \frac{x - iy}{x ^2 + y^2} = \frac{x}{x^2 + y^2} + i(\frac{-y}{x^2 + y^2})
$$

# 8

