$$
\newcommand\Dt{\Delta{t}}
\newcommand\Dtp{\Delta{t'}}
\newcommand\invgam{\sqrt{1 - \frac{v^2}{c^2}}}
\newcommand\gam{\frac{1}{\invgam}}
$$

### Problem 1

Call the average $K_s^0$ lifetime of for a kaon at rest $\Delta{t}$. Then, the lifetime for moving kaon at speed $v$ in the perspective of a rest observer $\Delta{t'}$ is:

$$
\Dtp = \gamma\Dt = \frac{\Dt}{\invgam}
$$

and the distance travelled by kaon before it decayed $x$ is
$$
x = \Dtp \cdot v
$$
We know the value of $x$ and $\Dt$, solve the equation, we get:
$$
v = \sqrt{1 \over \frac{1}{c^2} + \frac{\Dt^2}{x^2}} = 2.8802\cdot 10^{10} \text{ cm/s}
$$


### Problem 2

Both photons arrives at $\frac{20}{c} = 20 \text{ nanosecs}$.

### Problem 3

(a) the length of the ship *Linear B* is $L' = \gamma L = \invgam L = 0.6 \cdot 2000 = 1200 \text{ feet}$. in the respective of the ship *Linear A*.

(b) the length of the ship *Linear A* is $L' = \gamma L = \invgam L = 0.6 \cdot 2000 = 1200 \text{ feet}$. in the respective of the ship *Linear B*.

(c) the time takes to reach the head of the ship *Linear B* is $t_h = \gamma \frac{L}{2} / (c - 0.8c) = 3000 \text{ nanosecs}$. the time takes to reach the tail of the ship $t_t = \gamma \frac{L}{2} / (c +0.8c) = 333.3 \text{ nanosecs}$. 

### Problem 4

(a) 

1. $(x', y', z') = R(-\omega\sin\omega t, \omega \cos \omega t, 0) $ and $(x'', y'', z'') = R(-\omega^2\cos\omega t, -\omega^2 \sin\omega t, 0)$

2. $(x', y', z') \cdot (x'', y'', z'') = R^2(\omega^3\cos\omega t \sin\omega t - \omega^3 \cos\omega t \sin\omega t + 0) = 0$. The dot product between the velocity and acceleration is 0, so they are perpendicular.

(b)

1. 
   $$
   \begin{bmatrix}
   	2 & 1 \\
   	3 & 5
   \end{bmatrix} 
   \begin{bmatrix}
   	3 & 4 \\
   	2 & 1
   \end{bmatrix}
   = \begin{bmatrix}
   	8 & 9 \\
   	19 & 17
   \end{bmatrix}
   $$

2. $$
   \begin{bmatrix}
   	2 & 1 \\
   	3 & 5
   \end{bmatrix} 
   \begin{bmatrix}
   	5 \\
   	7
   \end{bmatrix}
   = \begin{bmatrix}
   	17 \\
   	50
   \end{bmatrix}
   $$

3. $$
   \begin{bmatrix}
   	6 & 2 \\
   \end{bmatrix} 
   \begin{bmatrix}
   	2 & 1 \\
   	3 & 5
   \end{bmatrix}
   = \begin{bmatrix}
   	18 & 16 \\
   \end{bmatrix}
   $$

4. 
   $$
   \begin{bmatrix}
   	2 & 4 \\
   \end{bmatrix}
   \begin{bmatrix}
   	2 & 1 \\
   	3 & 5
   \end{bmatrix} 
   \begin{bmatrix}
   	5 \\
   	7
   \end{bmatrix}
   = 234
   $$

5. $$
   \begin{bmatrix}
   	2 & 4 \\
   \end{bmatrix}
   \begin{bmatrix}
   	5 \\
   	7
   \end{bmatrix}
   = 38
   $$

6. $$
   \begin{bmatrix}
   	5 \\
   	7
   \end{bmatrix}
   \begin{bmatrix}
   	2 & 4 \\
   \end{bmatrix}
   = \begin{bmatrix}
   	10 & 20 \\
   	14 & 28
   \end{bmatrix}
   $$

   
