$$
\newcommand\rt{\vec{r}(t)}
\newcommand\tt{t^2}
\newcommand\ttt{t^3}
\newcommand\t[1]{t^#1}
\newcommand\ex{\vec{e}_x}
\newcommand\ey{\vec{e}_y}
\newcommand\ez{\vec{e}_z}
\newcommand\er{\vec{e}_r}
\newcommand\e[1]{\vec{e}_#1}

\newcommand\aone{\alpha_1}
\newcommand\atwo{\alpha_2}
\newcommand\athr{\alpha_3}
\newcommand\vt{\vec{v}(t)}
\newcommand\deri[2]{\frac{\d#1}{\d#2}}
\newcommand\derit[1]{\deri{#1}{t}}
\newcommand\deritn{\derit{}}
\newcommand\at{\vec{a}(t)}

\newcommand\vt{\vec{v}(t)}
\newcommand\ats{\vec{a}â€™(t)}
\newcommand\dvt{\dot{v}(t)}
\newcommand\drt{\dot{r}(t)}
\newcommand\ddrt{\ddot{r}(t)}
\newcommand\dvts{\dot{v}'(t)}
\newcommand\drts{\dot{r}'(t)}
\newcommand\ddrts{\ddot{r}'(t)}
\newcommand\ux{U(x)}
\newcommand\derix[1]{\deri{#1}{x}}
\newcommand\xx{x^2}
\newcommand\xxx{x^3}
\newcommand\half{{1\over2}}
\newcommand\pderi[2]{\frac{\part #1}{\part #2}}
\newcommand\pderin[1]{\pderi{}{#1}}
\newcommand\a{\alpha}
\newcommand\ao{\alpha_1}
\newcommand\at{\alpha_2}
\newcommand\const{\text{const}}
\newcommand\d{\text{d}}
\newcommand\invfrac[1]{\frac{1}{#1}}
$$

#### Question 1: Rocket in the atmosphere

>A rocket travels horizontally through the atmosphere and experiences a linear drag force $F_{drag} = -kv$, where $k > 0$ is a constant. Let $m_i$ be the initial mass of the rocket plus fuel and let $m_f$ be the final mass of the rocket after all fuel has burned. Let $u$ be the speed of the fuel relative to the rocket. Assume that all other external forces are negligible, i.e., ignore gravity.

##### (a)

>Write down the differential equation of motion, i.e, Newton's 2nd law

From the Lecture 05 Notes:
$$
\begin{align}
dp &= p_f - p_i \\ 
&= (M - \d m)(v + \d v) + \d m(v - u) - Mv \\ 
&= Mv + M\d v - v\d m -\d m\d v + v\d m - u\d m - Mv \\
&= M\d v  - u\d m
\end{align}
$$
Thus

#####   (b)

>The rocket burns a fuel at a constant rate $\derit{M} = -\a = \const$. Assume that the rocket starts from rest. Determine the final speed of the rocket in terms of $m_i$, $m_f$, $\alpha$, $u$ and $k$.

We know that $\derit{m} = -\derit{M} = \a$, and notice $M(t)$ depends on time. 
$$
\derit{M} = -\a \\
\int_{m_i}^{m(t)}\d M = -\int_{0}^{t} \a \d t \\
M(t) = m_i -\a t
$$
and thus 
$$
\begin{align}
-kv &= M\derit{v} - u\derit{m} \\
-kv &= M\derit{v} - u\a \\
u\a - kv &= M\derit{v} \\
\invfrac{M} \d t &= \frac{\d v}{u\a - kv} \\
\int_0^{t} \invfrac{m_i - \a t} \d s &= \int_{v(0)}^{v(t)} \frac{\d v}{u\a - kv} \\
-\invfrac \a \ln (m_i -\a t)\vline^t_0 &= -\invfrac k \ln (u\a - kv)\vline^{v(t)}_{v(0)} \\
k\ln(\frac{m_i - \a t}{m_i}) &=\a \ln(\frac{u\a - kv}{u\a - kv_0}) \\
\left (\frac{m_i -\a t}{m_i} \right )^k &= \left (\frac{u\a - kv}{u\a - kv_0} \right )^\a 
\end{align}
$$
$M(t_f) = m_f = m_i - \a t_f$ and thus $\a t = m_i - m_f$
$$
\left(\frac{m_f}{m_i} \right)^{k} = \left (\frac{u\a - kv}{u\a - kv_0} \right )^\a \\
\left(\frac{m_f}{m_i} \right)^{k \over \a} = \frac{u \a - kv}{u\a - kv_0} \\
(u\a -kv_0)\left(\frac{m_f}{m_i} \right)^{k \over \a} = u\a - kv \\
\fbox{$v = \invfrac{k} \left(u\a - (u\a -kv_0)\left(\frac{m_f}{m_i} \right)^{k \over \a}\right)$}
$$

#### Question 2: Particle motion

>A particle of mass $m$ moves in 3D in response to the force field
>$$
>\vec F(\vec r) = Az^2 \ex + Ay^3 \ey + 2Axz\ez
>$$

##### (a)

>Show that $\vec F$ is a conservative force and determine the potential energy.

$$
\pderi{F_x}{y} = 0 = \pderi{F_y}{x} \\
\pderi{F_x}{z} = 2Az  = \pderi{F_z}{x} \\
\pderi{F_y}{z} = 0 = \pderi{F_z}{y}
$$

So, exist $-\grad U = F$.
$$
U = \int -F_x \d x = -Az^2x +\phi_1(y, z) \\
$$

$$
\pderi{U}{y} = \pderi{\phi_1(y, z)}{y} = -Ay^3
$$

$$
\pderi{U}{z} = -2Axz + \pderi{\phi_1(y, z)}{z} = -2Axz \\
$$

$$
\phi_1(y,z) = \int Ay^3 \d y = -\frac{Ay^4}{4} + \psi_1(z)
$$

$$
\pderi{\phi_1(y, z)}{z} = \pderi{\psi_1(z)}{z} = 0
$$

$$
\phi_1(y, z) = -\frac{1}{4}Ay^4 + C_1
$$

$$
\fbox{$U = -Az^2x - \frac{1}{4}Ay^4 + C_1$}
$$

##### (b)

$$
E = T_0 + U_0 = T_f + U_f
$$

$$
\begin{align}
T_f - T_0 &= U_0 - U_f \\
&= U(0, 0, 0) - U(-1, 2, 1) \\ 
&= 0 - (-A\cdot 1^2 \cdot (-1) - \frac{1}{4}A\cdot(2)^4) \\
&= -A +4A \\
&= 3A
\end{align}
$$

$$
\half mv^2 = \half mv_0^2 + 3A \\
v^2 = v_0^2 + \frac{6A}{m} \\
\fbox{$v = \sqrt{v_0^2 + \frac{6A}{m}}$}
$$

#### Question 3: Nuclear forces and Yukawa potential


$$
f(r) = -\deri{V}{r} = -K(-\a e^{-\a r} r^{-1} + (-1)\cdot r^{-2}e^{-\a r}) = \a K \frac{e^{-\a r}}{r} + K\frac{e^{-\a r}}{r^2}
$$

$$
U_{\text{eff}} = \frac{L^2}{2mr^2} + \frac{Ke^{-\a r}}{r}
$$

We want to find the critical point of the $U_{\text{eff}}$:
$$
\deri{U}{r}  = -\frac{L^2}{mr^3} - K\invfrac {e^{\a r}}(\frac{\a}{r} + \invfrac{r^2})
$$

$$
\lim_{r \to 0} U_{\text{eff}}  = \infin \quad \lim_{r \to \infin}U_{\text{eff}} = 0
$$

We want to let $\deri{U}{r} = 0$, for $r > 0$
$$
\frac{L^2}{mr^3} = -Ke^{-\a r}(\frac{\a}{r} + \frac{1}{r^2}) \\
-\frac{L^2}{Km} = e^{-\a r}(\a r^2 + r)
$$
but the above equation seems unsolvable:

![image-20220922212517830](PHYS325HW3.assets/image-20220922212517830.png)

So, we will examine the property of $y = e^{-\a r}(\a r^2 + r)$
$$
\deri{y}{r} = e^{-\a r}(1+2\a r) - \a e^{-\a r}(r + \a r^2)
$$
Set the $\deri{y}{r} = 0$, we find
$$
\a^2 r^2 - \a r -1 = 0 \\
r = \frac{1 \pm \sqrt 5}{2\a}
$$
Since $\a \ge 0$, we know that there is only one root (one critical point for $y$) when $r > 0$. For $y$
$$
\lim_{r \to 0} y = 0 \quad \lim_{r \to \infin} y = 0 \quad y(r) > 0 \ \text{for}\  (r>0)
$$
That means $y$ will start $0$, goes to a maximum, and then approach to $0$, which looks roughly like:

![photo_2022-09-23_10-25-26](PHYS325HW3.assets/photo_2022-09-23_10-25-26.jpg)

So, for the original $\deri{U}{r} = 0$, there are few situations:

1. , $-\frac{L^2}{Km} > \max( e^{-\a r}(\a r^2 + r))$, as indicated by the green line, there is no solution for $\deri{U}{r} = 0$, and thus no critical point for $U$, and it will decrease from $\infin$ to $0$ monotonically, in this case, particles will always repulse from the origin and goes to infinity.
2. $-\frac{L^2}{Km} = \max( e^{-\a r}(\a r^2 + r))$, as indicated by the orange line, there is single solution for $\deri{U}{r} = 0$, and $\deri{U}{r} < 0$ for all $r > 0$ except when $-\frac{L^2}{Km} = e^{-\a r}(\a r^2 + r)$. That means there is one inflection point for $U$, and except the inflection point, $U$ will decrease from $\infin$ to $0$. In this case, there is a semi-stable equilibrium point where  $-\frac{L^2}{Km} = e^{-\a r}(\a r^2 + r)$ holds, when there is small disturbance, the particle will quickly goes to $r = \infin$.
3. $-\frac{L^2}{Km} < \max( e^{-\a r}(\a r^2 + r))$, as indicated by the blue line, there are two solutions for $\deri{U}{r}$, which means there are one maximum and minimum point for $U$. In this case $U$ will first decrease from $\infin$ to a minimum point, then increase to a maximum point, and eventually approaches to 0. In this case, there is a energy valley where particle could be trapped in, and make periodic motion in it., there is also an unstable equilibrium (the maximum) where the particle will either quickly go to $r = \infin$ or trapped in the energy valley if there is small disturbance.

##### (c)

That means $\deri{U}{r} = 0$ so that particle could have orbit will fixed radius
$$
L = \sqrt{-Kme^{-\a r}(\a a^2 + a)}
$$
and the energy is thus
$$
E = U_{\text{eff}} = \frac{L^2}{2mr^2} + \frac{Ke^{-\a r}}{r} = \frac{-Kme^{\a a}(\a a^2 + a)}{2ma^2} + \frac{Ke^{-\a a}}{a} \\ = \frac{-Ke^{-\a a}(\a a + 1)}{2a} + \frac{Ke^{-\a a}}{a} = \frac{Ke^{-\a a}}{a}(-\frac{\a a + 1}{2} + 1) = \frac{Ke^{-\a a}}{a}(\frac{-\a a +1}{2}) \\ = \frac{Ke^{-\a a}}{2a}(1 -\a a)
$$

##### (d)

$$
L = m\omega a^2 =\sqrt{-Kme^{-\a a}(\a a^2 + a)} \\
\omega = \sqrt{\frac{-Kme^{-\a a}(\a a^2 + a)}{m^2a^4}} = \sqrt{\frac{-Ke^{-\a a}(\a a + 1)}{ma^3}}
$$

##### (e)

$$
\frac{\d^2 U }{\d r^2}  = \frac{3L^2}{mr^4}+Ke^{-\a r}(\frac{2}{r^3} + \frac{2\a}{r^2} + \frac{\a ^2}{r})
$$

$$
\omega_{r} = \sqrt{\frac{U''(a)}{m}} = \sqrt{\frac{3L^2}{m^2a^4} + \frac{K}{m}e^{-\a a}(\frac{2}{a^3} + \frac{2\a}{a^2} + \frac{\a ^2}{a})} \\ = \sqrt{\frac{3\cdot -Kme^{-\a a}(\a a^2 + a)}{m^2a^4} + \frac{K}{m}e^{-\a a}(\frac{2}{a^3} + \frac{2\a}{a^2} + \frac{\a ^2}{a})} \\
=  \sqrt{\frac{K}{m}e^{-\a a} \frac{-3(\a a^2 + a)}{a^4} + \frac{K}{m}e^{-\a a}(\frac{2}{a^3} + \frac{2\a}{a^2} + \frac{\a ^2}{a})} \\
= \sqrt{\frac{K}{m}e^{-\a a} \left(\frac{-3\a a -1}{a^3} + \frac{2\a}{a^2} + \frac{\a ^2}{a}\right)}
$$

#### Question 4

$$
\int_{M}  -{G \d m \over r} = \int_{-{L \over 2}}^{L \over 2} -\lambda \frac{G}{\sqrt{y^2 + x^2}}\d x = -\lambda G \int_{-{L \over 2}}^{L \over 2}\frac{\d x}{\sqrt{x^2 + y^2}} = -\lambda G \cdot \left.\ln(x + \sqrt{x^2 + y^2})\right|_{-\frac{L}{2}}^{\frac{L}{2}} = \\ -\frac{GM}{L}\cdot\ln(\frac{\frac{L}{2} + \sqrt{\frac{L^2}{4} + y^2 }}{-\frac{L}{2} + \sqrt{\frac{L^2}{4} + y^2}}) = \\
-\frac{GM}{L}\cdot\ln(\frac{
	\left(\frac{L}{2} + \sqrt{\frac{L^2}{4} + y^2 }\right)^2
}{y^2 + \frac{L^2}{4} - \frac{L^2}{4}}) = -\frac{2GM}{L}\cdot \ln(\frac{\frac{L}{2} + \sqrt{\frac{L^2}{4}+y^2}}{y})
$$

When $y \gg L$, $y^2 \gg L^2$
$$
\Phi = -\frac{2GM}{L}\cdot \ln(\frac{\frac{L}{2} + \sqrt{\frac{L^2}{4}+y^2}}{y}) \\
= -\frac{2GM}{L}\cdot \ln(\frac{\frac{L}{2} + \sqrt{y^2}}{y}) \\
= -\frac{2GM}{L}\cdot \ln(\frac{L}{2y} + 1) \\
$$
Since $y \gg L$ and $\frac{L}{2y} \approx 0$, $\ln(\frac{L}{2y} + 1) \approx \frac{L}{2y}$
$$
\Phi \approx -\frac{2GM}{L} \cdot \frac{L}{2y} = -\frac{GM}{y}
$$

#### Question 5



